feat(data/fintype): add choose_unique and construct inverses to bijections (#421)

data/finset.lean
@@ -1593,6 +1593,23 @@ def attach_fin (s : finset ℕ) {n : ℕ} (h : ∀ m ∈ s, m < n) : finset (fin
 @[simp] lemma card_attach_fin {n : ℕ} (s : finset ℕ) (h : ∀ m ∈ s, m < n) :
   (s.attach_fin h).card = s.card := multiset.card_pmap _ _ _
 
+section choose
+variables (p : α → Prop) [decidable_pred p] (l : finset α)
+
+def choose_x (hp : (∃! a, a ∈ l ∧ p a)) : { a // a ∈ l ∧ p a } :=
+multiset.choose_x p l.val hp
+
+def choose (hp : ∃! a, a ∈ l ∧ p a) : α := choose_x p l hp
+
+lemma choose_spec (hp : ∃! a, a ∈ l ∧ p a) : choose p l hp ∈ l ∧ p (choose p l hp) :=
+(choose_x p l hp).property
+
+lemma choose_mem (hp : ∃! a, a ∈ l ∧ p a) : choose p l hp ∈ l := (choose_spec _ _ _).1
+
+lemma choose_property (hp : ∃! a, a ∈ l ∧ p a) : p (choose p l hp) := (choose_spec _ _ _).2
+
+end choose
+
 theorem lt_wf {α} [decidable_eq α] : well_founded (@has_lt.lt (finset α) _) :=
 have H : subrelation (@has_lt.lt (finset α) _)
     (inv_image (<) card),
